theories/rust_typing/existentials.v
@@ -168,6 +168,7 @@ Section ex.
   Next Obligation.
     iIntros (ty ? π r v) "(%x & HP & Hs)". by iApply ty_shr_sidecond.
   Qed.
+  Next Obligation. unfold TCNoResolve. apply _. Qed.
   Next Obligation.
     iIntros (ty κ π l r) "(%x & HP & Hv)". by iApply ty_shr_aligned.
   Qed.
